GebTests/Prototypes.lean
@@ -24,6 +24,7 @@ import GebTests.Prototypes.FreeTopos.InternalBenchmark
 import GebTests.Prototypes.FreeTopos.InternalCoproducts
 import GebTests.Prototypes.FreeTopos.InternalDerivation
 import GebTests.Prototypes.FreeTopos.InternalLogic
+import GebTests.Prototypes.FreeTopos.InternalRoseTrees
 import GebTests.Prototypes.FreeTopos.Prover
 import GebTests.Prototypes.Kernel
 import GebTests.Prototypes.LargeIR
